<?xml version="1.0" encoding="UTF-8"?>

<section>
  <title>October 3</title>

  
  <slide>
    <title>A totally real and not made up problem</title>
    
    <p>
      A rancher observes that, on average, for every 25 additional bales of hay produced in her fields,
      the population of her cattle herd increases by 4.
    </p>

    <p>
      She also knows that for every additional 10 mm of rain in a growing season, she will produce 75 more bales of hay.
    </p>

    <p>
      Recent weather patterns have seen rainfall increase by an average of 5 mm per year.
    </p>

    <p>
      At what rate (per year) is the size of her herd changing?
      <ol marker="A.">
        <li>
          <p>
            6 cows per year
          </p>
        </li>

        <li>
          <p>
            <m>\dfrac{8}{75}</m> of a cow per year
          </p>
        </li>

        <li>
          <p>
            <m>\dfrac53</m> of a cow per year
          </p>
        </li>

        <li>
          <p>
            About 234 cows per year
          </p>
        </li>
      </ol>
    </p>
  </slide>

  <slide>
    <title>Composing linear functions</title>
    
    <p>
      Let <m>f(x)=3(x-4)+5</m> and let <m>g(x)=-7x+4</m>
    </p>

    <p>
      What function is <m>f(g(x))</m>?
      <ol marker="A.">
        <li>
          <p>
            <m>-21(x-4)-24</m>
          </p>
        </li>
        <li>
          <p>
            <m>-21x-5</m>
          </p>
        </li>

        <li>
          <p>
            <m>-21x+5</m>
          </p>
        </li>

        <li>
          <p>
            <m>-21(x-4)+17</m>
          </p>
        </li>
      </ol>
    </p>

    <p pause="yes">
      What is the derivative of <m>f(g(x))</m>?
    </p>

    <p pause="yes">
      How is it related to the derivatives of <m>f(x)</m> and <m>g(x)</m>?
    </p>
  </slide>

  <slide>
    <title>The concept of the chain rule</title>
    
    <p>
      Derivatives represent rates of change.
    </p>

    <p>
      When one quantity depends on another, the rates at which they are changing are multiplied.
    </p>
    
    <image source="composition.svg" width="80%">
      <description></description>
    </image>
  </slide>

  <slide>
    <title>The chain rule</title>
    
    <theorem>
      <statement>
        <p>
          If <m>g</m> is differentiable at <m>x</m>,
          and <m>f</m> is differentiable at <m>g(x)</m>,
          then <m>h=f\circ g</m> is differentiable at <m>x</m>, and
          <me>
            h'(x) = \dfrac{d}{dx}(f(g(x))) = f'(g(x))g'(x)
          </me>.          
        </p>
      </statement>
    </theorem>
  </slide>

  <slide>
    <title>OK, let's try this thing</title>
    
    <p>
      Find the derivative of the following functions:
    </p>

    <p>
      <ol>
        <li>
          <p>
            <m>h(x)=e^{\sqrt{x}}</m>
          </p>
        </li>

        <li>
          <p>
            <m>k(x)=\sqrt{e^x}</m>
          </p>
        </li>

        <li>
          <p>
            <m>p(x)=\sin(x^4)</m>
          </p>
        </li>
        <li>
          <p>
            <m>q(x)=\sin^4(x)</m>
          </p>
        </li>
      </ol>
    </p>
  </slide>

  <slide>
    <title>Example: derivative of <m>\sec(x)</m></title>
    
    <p>
      We know the derivatives of <m>\sin(x)</m> and <m>\cos(x)</m>.
    </p>

    <p>
      What about their reciprocals, <m>\csc(x)</m> and <m>\sec(x)</m>?
    </p>

    <p pause="yes">
      Observe that <m>\sec(x) = \dfrac{1}{\cos(x)}=(\cos(x))^{-1}</m>
    </p>

    <p pause="yes">
      <alert>Caution!!</alert> <m>(\cos(x))^{-1}</m> is not the same thing as <m>\cos^{-1}(x)</m>!
      (Even though <m>(\cos(x))^2</m> is the same thing as <m>\cos^2(x)</m>...)
    </p>

    <p pause="yes">
      By the chain rule, <m>\dfrac{d}{dx}(\sec(x))=\dfrac{d}{dx}(\cos(x))^{-1}=-1(\cos(x))^{-2}(-\sin(x))</m>
    </p>

    <p pause="yes">
      We can clean this up: <m>-1(\cos(x))^{-2}(-\sin(x))=\dfrac{\sin(x)}{\cos^2(x)}=\sec(x)\tan(x)</m>
    </p>
  </slide>

  <slide>
    <title>Goodbye, cruel quotient rule!</title>
    
    <p>
      It may be helpful to observe that <m>\dfrac{f(x)}{g(x)}=f(x)(g(x))^{-1}</m>.
    </p>
  </slide>

  <slide>
    <title><m>x^a</m> and <m>a^x</m></title>
    
    <p>
      Technically, we've only demonstrated the power rule for the dervative of <m>x^n</m>, 
      when <m>n=1, 2, 3, \ldots</m> 
    </p>

    <p>
      Recall the following two facts about logarithms:
      <ol>
        <li>
          <p>
            <m>\ln(p^q)=q\ln(p)</m>
          </p>
        </li>

        <li>
          <p>
            Since <m>\ln(x)</m> is the inverse of <m>e^x</m>,
            <m>\ln(e^x)=x</m> and <m>e^{\ln(x)}=x</m>.
          </p>
        </li>
      </ol>
    </p>

    <p>
      If <m>f(x)=x^a</m> and <m>g(x)=a^x</m>, then:
      <ol marker="A.">
        <li>
          <p>
            <m>f(x)=e^{a\ln(x)}</m> and <m>g(x)=e^{x\ln(a)}</m>
          </p>
        </li>

        <li>
          <p>
            <m>f(x)=e^{x\ln(a)}</m> and <m>g(x)=e^{a\ln(x)}</m>
          </p>
        </li>

        <li>
          <p>
            <m>f(x)=\ln(e^{ax})</m> and <m>g(x)=\log_a(a^{ex})</m>
          </p>
        </li>
      </ol>
    </p>
  </slide>
</section>