<?xml version="1.0" encoding="UTF-8"?>

<section>
  <title>October 17</title>

  <slide>
    <title>From last time...</title>
    
    <p>
      Technically, we've only demonstrated the power rule for the dervative of <m>x^n</m>, 
      when <m>n=1, 2, 3, \ldots</m> 
    </p>

    <p>
      Recall the following two facts about logarithms:
      <ol>
        <li>
          <p>
            <m>\ln(p^q)=q\ln(p)</m>
          </p>
        </li>

        <li>
          <p>
            Since <m>\ln(x)</m> is the inverse of <m>e^x</m>,
            <m>\ln(e^x)=x</m> and <m>e^{\ln(x)}=x</m>.
          </p>
        </li>
      </ol>
    </p>

    <p>
      <ul>
        <li>
          <p>
            For <m>f(x)=x^a</m>, <m>f(x)=e^{\ln(x^a)}=e^{a\ln(x)}</m>. Therefore,
            <me>
              f'(x) = \frac{d}{dx}e^{a\ln(x)} = e^{a\ln(x)}\frac{d}{dx}(a\ln(x)) = x^a\left(\frac{a}{x}\right) = ax^{a-1}
            </me>
            
          </p>
        </li>

        <li>
          <p>
            For <m>g(x)=a^x</m>, <m>g(x)=e^{\ln(a^x)} = e^{x\ln(a)}</m>. Therefore,
            <me>
              g'(x) = \frac{d}{dx}(e^{x\ln(a)}) = e^{x\ln(a)}\frac{d}{dx}(\ln(a)x) = a^x\ln(a)
            </me>
            
          </p>
        </li>
      </ul>
    </p>
  </slide>

  <slide>
    <title>Harder chain rule</title>
    
    <p>
      Note: using the quotient rule,
      <me>
        \frac{d}{dx}\tan(x) = \frac{d}{dx}\left(\frac{\sin(x)}{\cos(x)}\right)=\frac{\cos(x)\cos(x)-(-\sin(x))\sin(x)}{\cos^2(x)}=\frac{1}{\cos^2(x)}=\sec^2(x)
      </me>
      
    </p>

    <p>
      <em>Exercise:</em> what is the derivative of <m>f(x) = \tan(\sqrt{x^4+1})</m>?
    </p>

    <p>
      <ol marker="A.">
        <li>
          <p>
            <m>f'(x)=\sec^2(\sqrt{x^4+1})</m>
          </p>
        </li>

        <li>
          <p>
            <m>f'(x)=4x^3\sec^2(\sqrt{x^4+1})</m>
          </p>
        </li>

        <li>
          <p>
            <m>f'(x)=\sec^2(\sqrt{x^4+1})\left(\frac12(x^4+1)^{-1/2}\right)(4x^3)</m>
          </p>
        </li>

        <li>
          <p>
            <m>f'(x)=\sec^2\left(\frac{2x^3}{\sqrt{x^4+1}}\right)</m>
          </p>
        </li>
      </ol>
    </p>
  </slide>

  <slide>
    <title>Products, and quotients, and chain rule, oh my!</title>
    
    <p>
      What is the derivative of <m>f(x) = \dfrac{e^{x^3}\sin^2(x)}{\sqrt{x^2+1}}</m>?
    </p>

    <p>
      <ol marker="A.">
        <li>
          <p>
            <m>f'(x) = \dfrac{(3x^2e^{x^3}\sin^2(x)+2e^{x^3}\sin(x)\cos(x))\sqrt{x^2+1}-e^{x^3}\sin^2(x)\left(x(x^2+1)^{-1/2}\right)}{x^2+1}</m>
          </p>
        </li>
        <li>
          <p>
            <m>f'(x) = \dfrac{(3x^2e^{x^3}\sin^2(x)+e^{x^3}\cos^2(x))\sqrt{x^2+1}-e^{x^3}\sin^2(x)\left(x(x^2+1)^{-1/2}\right)}{x^2+1}</m>
          </p>
        </li>
        <li>
          <p>
            <m>f'(x) = \dfrac{(3x^2e^{x^3}\sin^2(x)+2e^{x^3}\cos(x))\sqrt{x^2+1}-e^{x^3}\sin^2(x)\left(\frac{1}{2}(x^2+1)^{-1/2}\right)}{x^2+1}</m>
          </p>
        </li>
        <li>
          <p>
            <m>f'(x) = \dfrac{(e^{x^3}\sin^2(x)+2e^{x^3}\sin(x)\cos(x))\sqrt{x^2+1}-e^{x^3}\sin^2(x)\left(\frac{x}{\sqrt{x^2+1}}\right)}{x^2+1}</m>
          </p>
        </li>
      </ol>
    </p>
  </slide>

  <slide>
    <title>Sometimes, logarithms are our friends</title>
    
    <p>
      For any function <m>f(x)</m>, let <m>g(x)=\ln(f(x))</m>. Recall that the derivative of <m>\ln(x)</m> is <m>\dfrac1x</m>.
    </p>

    <p>
      By the chain rule,
      <me>
        g'(x) = \frac{d}{dx}\ln(f(x)) = \frac{1}{f(x)}\frac{d}{dx}f(x) = \frac{f'(x)}{f(x)}
      </me>.
      
    </p>

    <p>
      Consider the function <m>f(x) = \dfrac{e^{x^3}\sin^2(x)}{\sqrt{x^2+1}}</m> from the last slide.
    </p>

    <p>
      Using log properties,
      <md>
        <mrow>\ln(f(x)) \amp = \ln\left(\frac{e^{x^3}\sin^2(x)}{\sqrt{x^2+1}}\right) = \ln(e^{x^3}\sin^2(x))-\ln(\sqrt{x^2+1})</mrow>
        <mrow> \amp = \ln(e^{x^3})+\ln(\sin^2(x))-\ln((x^2+1)^{1/2})= x^3+2\ln(\sin(x))-\frac12\ln(x^2+1)</mrow>
      </md>
    </p>

    
  </slide>

  <slide>
    <title>Friendly logarithms, continued</title>
    
    <p>
      From the last slide, we found that <m>\dfrac{d}{dx}\ln(f(x))=\dfrac{f'(x)}{f(x)}</m>, and
      <me>
        \ln(f(x)) = x^3+2\ln(\sin(x))-\frac12\ln(x^2+1)
      </me>.
      
    </p>
    <p>
      Taking the derivative of both sides, we get:
      <me>\frac{f'(x)}{f(x)} = 3x^2+2\frac{\cos(x)}{\sin(x)}-\frac12\frac{2x}{x^2+1}</me>
    </p>


    <p>
      Now multiply both sides by <m>f(x) = \dfrac{e^{x^3}\sin^2(x)}{\sqrt{x^2+1}}</m> and we get:
      <me>
        f'(x) = \frac{e^{x^3}\sin^2(x)}{\sqrt{x^2+1}}\left(3x^2+2\frac{\cos(x)}{\sin(x)}-\frac12\frac{2x}{x^2+1}\right)
      </me>
      
    </p>
  </slide>

  <slide>
    <title>Logarithmic differentiation</title>
    
    <p>
      Let <m>f(x) = (4+x^2)^{3x}</m>. Find <m>f'(x)</m> by computing the derivative of <m>\ln(f(x))</m>.
    </p>

    <p>
      The derivative of <m>f(x)</m> is:
      <ol marker="A.">
        <li>
          <p>
            <m>f'(x)=3\ln(4+x^2)+\dfrac{6x^2}{4+x^2}</m>
          </p>
        </li>

        <li>
          <p>
            <m>f'(x)=(4+x^2)^{3x}\left(3\ln(4+x^2)+\dfrac{6x^2}{4+x^2}\right)</m>
          </p>
        </li>

        <li>
          <p>
            <m>f'(x)=3x(4+x^2)^{3x-1}</m>
          </p>
        </li>

        <li>
          <p>
            <m>f'(x) = (4+x^2)^{3x}\ln(4+x^2)</m>
          </p>
        </li>
      </ol>
    </p>
  </slide>

  <slide>
    <title>Implicit differentiation</title>

    <p>
      According to the chain rule, <m>\dfrac{d}{dx}f(g(x))=f'(g(x))g'(x)</m>.
    </p>

    <p>
      If we let <m>y=g(x)</m> and write <m>y'=g'(x)</m>, this becomes:
      <me>
        \frac{d}{dx}f(y) = f'(y)\,y'
      </me>.
      
    </p>

    <p>
      For example, <m>\dfrac{d}{dx}(y^2)=2y\,y'</m>, assuming that <m>y</m> is a function of <m>x</m>.
    </p>
    
    <p>
      This is called <em>implicit differentiation</em>.
    </p>
  </slide>

  <slide>
    <title>The classic example: a circle</title>
    
    <p>
      Consider the equation <m>x^2+y^2=4</m> (a circle). We say that it <term>implicitly defines</term>
      <m>y</m> as a function of <m>x</m>.
    </p>

    <p>
      This means we can (in principle) find a function <m>g(x)</m> so that <m>y=g(x)</m> satisfies the equation:
      <me>
        x^2+(g(x))^2=4
      </me>.
      
    </p>

    <p>
      The graph of <m>g(x)</m> won't give the <em>whole</em> circle. (Why?) We might need different functions near different points.
    </p>

    <p pause="yes">
      Can we find a function that works near the point <m>(0,2)</m>?
    </p>

    <p pause="yes">
      Can we find a function that works near the point <m>(1,-\sqrt{3})</m>?
    </p>

    <p pause="yes">
      Can we find a function that works near the point <m>(2,0)</m>?
    </p>
  </slide>

  <slide>
    <title>Finding <m>y'</m></title>
    
    <p>
      Use implicit differentiation to find <m>y'</m> if
      <me>
        x^2+y^2=4
      </me>.
      
    </p>

    <p>
      <ol marker="A.">
        <li>
          <p>
            <m>y'=\sqrt{4-x^2}</m>
          </p>
        </li>

        <li>
          <p>
            <m>y'=\sqrt{4-2x}</m>
          </p>
        </li>

        <li>
          <p>
            <m>y' = -\dfrac{x}{y}</m>
          </p>
        </li>

        <li>
          <p>
            <m>y' = \dfrac{2-x}{y}</m>
          </p>
        </li>
      </ol>
    </p>
  </slide>

  <slide>
    <title>A harder example</title>
    
    <p>
      Use implicit differentiation to find <m>y'</m> if
      <m>y</m> is implicitly defined as a function of <m>x</m>
      by the equation
      <me>
        \sin(xy)+xy^3=7
      </me>.
      
    </p>

    <p pause="yes">
      No poll this time -- try it for a few minutes, and then we'll solve it together.
    </p>
  </slide>

  <slide>
    <title>Tangent lines</title>
    
    <p>
      We can use implicit differentiation to find the equation of a tangent line at a given point on a curve.
    </p>

    <p>
      Example: find the equation of the tangent line to the curve given by the equation 
      <me>2x^2y^2+xy^3-x^2-4y^2=2</me>
      at the point <m>(2,1)</m>.
    </p>
  </slide>

  <slide>
    <title>One for you to try</title>
    
    <p>
      What is the equation of the tangent line to the curve
      <me>
        (x^2+y^2)^2=4xy
      </me>
      at the point <m>(1,1)</m>?
      
    </p>

    <p>
      <ol marker="A.">
        <li>
          <p>
            <m>y=1+1(x-1)</m>
          </p>
        </li>

        <li>
          <p>
            <m>y=-1+1(x-1)</m>
          </p>
        </li>

        <li>
          <p>
            <m>y=1-1(x-1)</m>
          </p>
        </li>

        <li>
          <p>
            <m>y=-1-1(x-1)</m>
          </p>
        </li>

        <li>
          <p>
            There is no tangent line
          </p>
        </li>

        <li>
          <p>
            That point isn't even on the curve, man!
          </p>
        </li>
      </ol>
    </p>
  </slide>
</section>